src/mapping/PStoRMWInit.v
@@ -76,10 +76,36 @@ Module PStoRMWInit.
 
   Variant sim_thread_init (tid: Ident.t) (th_ps: PSThread.t lang_ps) (eu: RMWExecUnit.t (A:=unit)): Prop :=
     | sim_thread_init_intro
+        (PROMISES_PS: PSLocal.promises (PSThread.local th_ps) = BoolMap.bot)
+        (FWD: forall loc, eu.(RMWExecUnit.local).(Local.fwdbank) loc = FwdItem.mk bot bot false)
+        (SIM_STATE: sim_state (PSThread.state th_ps) (RMWExecUnit.state eu))
+        (SIM_TVIEW: sim_tview (PSLocal.tview (PSThread.local th_ps)) (RMWExecUnit.local eu))
         (SIM_MEM: sim_memory_init tid
                                   (PSLocal.reserves (PSThread.local th_ps))
                                   (PSGlobal.memory (PSThread.global th_ps))
                                   (RMWExecUnit.mem eu))
+  .
+
+  Variant sim_thread_sl_init (tid: Ident.t) (gl_ps: PSGlobal.t) (mem_arm: Memory.t):
+    forall (sl_ps: {lang: language & Language.state lang} * PSLocal.t)
+           (sl_arm: RMWState.t (A:=View.t (A:=unit)) * Local.t (A:=unit)), Prop :=
+    | sim_thread_sl_init_intro
+        st_ps lc_ps st_arm lc_arm
+        (SIM_THREAD: sim_thread_init tid
+                       (PSThread.mk _ st_ps lc_ps gl_ps) (RMWExecUnit.mk st_arm lc_arm mem_arm)):
+      sim_thread_sl_init tid gl_ps mem_arm
+        (existT _ lang_ps st_ps, lc_ps) (st_arm, lc_arm)
+  .
+
+  Variant sim_init (c: PSConfiguration.t) (m: RMWMachine.t): Prop :=
+    | sim_init_intro
+        (SIM_THREADS:
+          forall tid,
+            opt_rel
+              (sim_thread_sl_init tid c.(PSConfiguration.global) m.(RMWMachine.mem))
+              (IdentMap.find tid c.(PSConfiguration.threads))
+              (IdMap.find tid m.(RMWMachine.tpool)))
+        (SIM_SC: c.(PSConfiguration.global).(PSGlobal.sc) = TimeMap.bot)
   .
 
   Definition ps_locations_only (mem: Memory.t): Prop :=
@@ -103,6 +129,26 @@ Module PStoRMWInit.
     i. des. eauto.
   Qed.
 
+  Lemma machine_promise_step_ps_locations_only
+        m1 m2
+        (LOCS: ps_locations_only m2.(RMWMachine.mem))
+        (STEP: RMWMachine.step RMWExecUnit.promise_step m1 m2):
+    ps_locations_only m1.(RMWMachine.mem).
+  Proof.
+    inv STEP.
+    hexploit promise_step_ps_locations_only; try exact STEP0; ss.
+  Qed.
+
+  Lemma rtc_machine_promise_step_ps_locations_only
+        m1 m2
+        (LOCS: ps_locations_only m2.(RMWMachine.mem))
+        (STEP: rtc (RMWMachine.step RMWExecUnit.promise_step) m1 m2):
+    ps_locations_only m1.(RMWMachine.mem).
+  Proof.
+    induction STEP; ss.
+    eapply machine_promise_step_ps_locations_only; try exact H. auto.
+  Qed.
+
   Lemma init_sim_memory_init tid:
     sim_memory_init tid PSMemory.bot PSMemory.init Memory.empty.
   Proof.
@@ -112,42 +158,51 @@ Module PStoRMWInit.
     - exploit PSMemory.init_get; eauto. i. des. subst. inv TO.
   Qed.
 
-  Lemma empty_loc_app
-        loc from to mem1 mem2
-        (TO: to <= S (length mem1))
-        (EMPTY: empty_loc loc from to mem1):
-    empty_loc loc from to (mem1 ++ mem2).
+  Lemma init_sim_init
+        prog_ps
+        prog_arm
+        (COMPILE: ps_to_rmw_program prog_ps prog_arm):
+    sim_init (Configuration.init (IdentMap.map (fun s => existT _ lang_ps s) prog_ps))
+             (RMWMachine.init prog_arm).
   Proof.
-    ii. eapply EMPTY; eauto.
-    rewrite List.nth_error_app1 in MSG; ss. nia.
+    econs; ss. i.
+    specialize (COMPILE tid).
+    unfold Threads.init.
+    rewrite IdentMap.Facts.map_o in *.
+    rewrite IdentMap.Facts.map_o in *.
+    rewrite IdMap.map_spec.
+    destruct (IdentMap.find tid prog_ps) eqn:FIND_PS,
+        (IdMap.find tid prog_arm) eqn:FIND_ARM; ss.
+    econs. econs. econs; ss.
+    - econs; ss. ii.
+      unfold RegFile.init.
+      rewrite IdentFun.init_spec.
+      unfold RMap.find, RMap.init.
+      rewrite IdMap.gempty. ss.
+    - econs; ss; refl.
+    - clear. econs; i.
+      + destruct ts; ss.
+        unfold Memory.get_msg in *. ss.
+        apply nth_error_some in GET_ARM. ss. nia.
+      + exploit PSMemory.init_get; eauto. i. des. subst. inv TO.
   Qed.
 
-  Lemma read_ts
-        loc ts mem val
-        (READ: Memory.read loc ts mem = Some val):
-    ts <= length mem.
+  Lemma reserve_step_future
+        lang loc from to (th1 th2: PSThread.t lang)
+        (STEP: PSThread.step (ThreadEvent.reserve loc from to) th1 th2):
+    (<<STATE: th1.(PSThread.state) = th2.(PSThread.state)>>) /\
+    (<<TVIEW: th1.(PSThread.local).(PSLocal.tview) = th2.(PSThread.local).(PSLocal.tview)>>) /\
+    (<<PRM: th1.(PSThread.local).(PSLocal.promises) = th2.(PSThread.local).(PSLocal.promises)>>) /\
+    (<<RSV: PSMemory.le th1.(PSThread.local).(PSLocal.reserves) th2.(PSThread.local).(PSLocal.reserves)>>) /\
+    (<<SC: th1.(PSThread.global).(Global.sc) = th2.(PSThread.global).(Global.sc)>>) /\
+    (<<GPRM: th1.(PSThread.global).(Global.promises) = th2.(PSThread.global).(Global.promises)>>) /\
+    (<<MEM: PSMemory.le th1.(PSThread.global).(Global.memory) th2.(PSThread.global).(Global.memory)>>).
   Proof.
-    unfold Memory.read in *.
-    destruct ts; ss; try nia. des_ifs.
-    exploit nth_error_some; eauto.
+    inv STEP; inv LOCAL. inv LOCAL0. inv RESERVE. ss.
+    splits; ss; eauto using PSMemory.add_le.
   Qed.
 
-  Lemma get_msg_ts
-        ts mem msg
-        (GET: Memory.get_msg ts mem = Some msg):
-    ts <= length mem.
-  Proof.
-    unfold Memory.get_msg in *.
-    destruct ts; ss.
-    exploit nth_error_some; eauto.
-  Qed.
-
-  Lemma incr_ntt_S ts: PSTime.incr (ntt ts) = ntt (S ts).
-  Proof.
-    ss.
-  Qed.
-
-  Lemma sim_memory_init_promise_step
+  Lemma sim_thread_init_promise_step
         tid th1_ps (eu1 eu2: RMWExecUnit.t (A:=unit))
         (SIM1: sim_thread_init tid th1_ps eu1)
         (LC_WF1_PS: PSLocal.wf (PSThread.local th1_ps) (PSThread.global th1_ps))
@@ -200,7 +255,11 @@ Module PStoRMWInit.
 
     esplits.
     { econs 1. econs 2. econs; eauto. }
-    { inv SIM_MEM. econs. ss. econs; i.
+    { inv SIM_MEM. econs; ss.
+      { destruct lc1_ps, lc1_arm. ss.
+        inv SIM_TVIEW. econs; ss.
+      }
+      econs; i.
       { exploit Memory.get_msg_snoc_inv; eauto. i. des.
         - exploit MEM_SOUND; eauto. i. des.
           exploit PSMemory.add_get1; try exact GET_PS; eauto. i.
@@ -248,5 +307,86 @@ Module PStoRMWInit.
           eapply nth_error_app_mon; eauto.
       }
     }
-  Qed.    
+  Qed.
+
+  Lemma sim_memory_init_other
+        tid rsv_ps mem1_ps mem_arm
+        tid' rsv_ps' mem2_ps mem_interference
+        (SIM1: sim_memory_init tid rsv_ps mem1_ps mem_arm)
+        (SIM_OTHER: sim_memory_init tid' rsv_ps' mem2_ps (mem_arm ++ mem_interference))
+        (INTERFERENCE: forall msg (IN: List.In msg mem_interference),
+            msg.(Msg.tid) <> tid)
+        (LE: PSMemory.le mem1_ps mem2_ps):
+    sim_memory_init tid rsv_ps mem2_ps (mem_arm ++ mem_interference).
+  Proof.
+    inv SIM1. inv SIM_OTHER. econs; eauto; i.
+    exploit Memory.get_msg_app_inv; eauto. i. des.
+    - exploit MEM_SOUND; eauto. i. des. esplits; eauto.
+      unguard. des; auto. right. esplits; eauto.
+      + eapply Memory.get_msg_mon; eauto.
+      + eapply empty_loc_app; ss. nia.
+    - exploit MEM_SOUND0; eauto. i. des.
+      esplits; eauto. i.
+      apply List.nth_error_In in x1.
+      exploit INTERFERENCE; eauto. ss.
+  Qed.
+
+  Lemma sim_init_promise_step
+        c1 (m1 m2: RMWMachine.t)
+        (SIM1: sim_init c1 m1)
+        (WF1_PS: PSConfiguration.wf c1)
+        (LOCS: ps_locations_only m2.(RMWMachine.mem))
+        (STEP: RMWMachine.step RMWExecUnit.promise_step m1 m2):
+    exists tid c2,
+      (<<STEP_PS: PSConfiguration.step MachineEvent.silent tid c1 c2>>) /\
+      (<<SIM2: sim_init c2 m2>>).
+  Proof.
+    destruct c1 as [ths1 gl1].
+    destruct m1 as [tpool1 mem1_arm], m2 as [tpool2 mem2_arm].
+    inv SIM1. inv STEP. ss. subst.
+    generalize (SIM_THREADS tid).
+    rewrite FIND. i. inv H. inv REL.
+    inv WF1_PS. inv WF. exploit THREADS; eauto. s. i.
+    clear DISJOINT THREADS PROMISES.
+    exploit sim_thread_init_promise_step; try exact SIM_THREAD; eauto; ss. i. des.
+    destruct th2_ps. esplits.
+    - replace MachineEvent.silent with
+        (ThreadEvent.get_machine_event (ThreadEvent.reserve loc from to)) by ss.
+      econs; eauto. ss. i.
+      econs 2; try refl. inv SIM2. ss.
+    - exploit reserve_step_future; eauto. s. i. des. subst.
+      econs; s; try congr. i.
+      rewrite IdentMap.gsspec, IdMap.add_spec.
+      do 2 condtac; try congr; subst.
+      + inv SIM_THREAD. ss. econs. econs. ss.
+      + specialize (SIM_THREADS tid0). inv SIM_THREADS.
+        { destruct (IdentMap.find tid0 ths1); ss. }
+        destruct (IdentMap.find tid0 ths1) eqn:FIND_PS'; ss. inv H0.
+        inv REL. econs. econs.
+        inv SIM_THREAD0. ss. econs; ss.
+        inv STEP0. inv LOCAL. inv MEM2. ss. subst.
+        inv SIM2. ss.
+        eapply sim_memory_init_other; eauto.
+        ii. inv IN; ss.
+  Qed.
+
+  Lemma sim_init_rtc_promise_step
+        c1 (m1 m2: RMWMachine.t)
+        (SIM1: sim_init c1 m1)
+        (WF1_PS: PSConfiguration.wf c1)
+        (LOCS: ps_locations_only m2.(RMWMachine.mem))
+        (STEPS: rtc (RMWMachine.step RMWExecUnit.promise_step) m1 m2):
+    exists c2,
+      (<<STEPS_PS: rtc PSConfiguration.tau_step c1 c2>>) /\
+      (<<SIM2: sim_init c2 m2>>).
+  Proof.
+    revert c1 SIM1 WF1_PS.
+    induction STEPS; i; eauto.
+    hexploit rtc_machine_promise_step_ps_locations_only; try exact STEPS; ss. i.
+    exploit sim_init_promise_step; try exact H; eauto. i. des.
+    exploit PSConfiguration.step_future; eauto. i. des.
+    exploit IHSTEPS; try exact SIM2; eauto. i. des.
+    esplits; [|eauto].
+    econs; eauto. econs. eauto.
+  Qed.
 End PStoRMWInit.
